LeanCats/Syntax.lean
@@ -54,15 +54,6 @@ syntax "empty" : assertion
 syntax "acyclic" : assertion
 syntax "~"assertion : assertion
 
-syntax "_" : name
-syntax "O" : name
-syntax "ext" : name
-syntax "FW" : name
-syntax "id" : name
-syntax "loc" : name
-syntax "narrower" : name
-syntax "wider" : name
-
 /- table events. -/
 syntax "W" : annotable_events -- write events
 syntax "R" : annotable_events -- read events
@@ -70,23 +61,28 @@ syntax "B" : annotable_events -- branch events
 syntax "F" : annotable_events -- fence events
 syntax "RMW" : annotable_events -- read-modify-write events
 syntax "SRCU" : annotable_events -- srcu events
+syntax "IW" : annotable_events -- initial writes
+syntax "M" : annotable_events -- memory events, M = W ∪ R
 
 syntax "___" : predefined_events -- all events
-syntax "IW" : predefined_events -- initial writes
-syntax "M" : predefined_events -- memory events, M = W ∪ R
 syntax annotable_events : predefined_events
 
 /- defined_relations: -/
 syntax "O" : predefined_relations -- empty relation
 syntax "rf" : predefined_relations -- read from
-syntax "rfe" : predefined_relations -- read from external
 syntax "fr" : predefined_relations -- from read
 syntax "co" : predefined_relations -- from read
 syntax "id" : predefined_relations -- identity
 syntax "loc" : predefined_relations -- same location
-syntax "ext" : predefined_relations -- external (different pids)
 syntax "po" : predefined_relations -- program order
 syntax "rmw" : predefined_relations -- read-modify-write
+syntax "mb" : predefined_relations -- read-modify-write
+syntax "data" : predefined_relations -- data dependencies, starts with a read
+syntax "ctrl" : predefined_relations -- control dependencies, starts with a read
+syntax "addr" : predefined_relations -- address dependencies, starts with a read
+syntax "rmb" : predefined_relations -- read memory barrier, read -> read
+syntax "wmb" : predefined_relations -- write memory barrier, write -> write
+syntax "fence" : predefined_relations -- fence barrier
 
 syntax keyword : dsl_term
 syntax num : dsl_term
@@ -104,12 +100,15 @@ syntax expr "&" expr : expr
 syntax expr ";" expr : expr
 syntax expr "\\" expr : expr
 syntax:60 expr:60 "*" expr:61 : expr
+syntax:70 expr "*" : expr -- Reflexive Transitive Closure.
+syntax:70 expr "+" : expr -- Transitive Closure.
 syntax expr "^" expr : expr
 syntax expr "+" expr : expr
 syntax expr "-" expr : expr
+syntax expr "?" : expr
 syntax:71 expr "^-1" : expr
 -- The procedure will return a value, so we can use it in the expression.
-syntax cat_ident "(" expr,* ")" : expr
+syntax dsl_term "(" expr,* ")" : expr
 
 syntax "[" expr "]" : expr
 
@@ -117,9 +116,10 @@ syntax assertion expr ("as" cat_ident)? : inst
 -- The flag is used to witness the assertion, so it doesn't change the states of the execution, we could just ignore it.
 syntax "flag" assertion expr "as" expr : inst
 syntax "let" cat_ident "=" expr : inst
+syntax "let" cat_ident "(" cat_ident,* ")" "=" expr : inst
 syntax "enum" cat_ident "=" sepBy(cat_ident, "||") : inst
 -- event class can be R W F B RMW or a custom name like SRCU
-syntax "instructions" annotable_events "[" expr "]" : inst
+syntax "instructions" "{" annotable_events,+ "}" "[" expr "]" : inst
 
 syntax "(*" ident* "*)" : inst
 syntax "include" str : inst
