LeanCats/TsoWeakerThanSc.lean
@@ -1,0 +1,38 @@
+import LeanCats.Macro
+import LeanCats.ModelReader
+import LeanCats.Data
+import LeanCats.Relations
+import LeanCats.Theorems
+import LeanCats.Basic
+
+defcat <"tso.cat">
+defcat <"sc.cat">
+
+theorem scvtso
+  (evts : Data.Events)
+  (X : CandidateExecution evts)
+  : sc.sc evts X → tso.tso evts X :=
+by
+  unfold sc.sc
+  simp
+  intro sc
+  apply ayclicMono sc
+  simp [CatRel.CatUnion.union] at *
+  intro a b h
+  rcases h with hImplied | h
+  · rcases hImplied with ⟨mid, hpo_amid, htail⟩
+    rcases htail with hId | hComp
+    · have hmid_eq_b : mid = b := hId.1
+      subst hmid_eq_b
+      exact Or.inl hpo_amid
+    · rcases hComp with ⟨x, hIdMidX, hpo_xb⟩
+      have hmid_eq_x : mid = x := hIdMidX.1
+      subst hmid_eq_x
+      exact Or.inl (X.prePo _ _ _ hpo_amid hpo_xb)
+  · rcases h with hxppo | h
+    · exact Or.inl hxppo.2
+    · rcases h with hrfe | h
+      · exact Or.inr (Or.inl hrfe.1)
+      · rcases h with hfr | hco
+        · exact Or.inr (Or.inr (Or.inl hfr))
+        · exact Or.inr (Or.inr (Or.inr hco))
